Move Clause stuff to HornClauses

common/theories/LoopChecking/HornClauses.v
@@ -5,10 +5,215 @@ From Stdlib Require Import Orders OrderedTypeAlt OrderedTypeEx MSetList MSetInte
 From MetaRocq.Utils Require Import utils.
 
 From MetaRocq.Common Require Universes.
+From MetaRocq.Common Require Import Interfaces.
 From Equations Require Import Equations.
 Set Equations Transparent.
 
 Ltac rw l := rewrite_strat (topdown l).
 Ltac rw_in l H := rewrite_strat (topdown l) in H.
 
+Module Clauses (LS : LevelSets).
+  Module Export FLS := FromLevelSets LS.
 
+  Notation univ := nonEmptyLevelExprSet.
+  Definition clause : Type := univ × LevelExpr.t.
+
+  Module Clause.
+
+  Definition t := clause.
+
+  Definition eq : t -> t -> Prop := eq.
+
+  Definition eq_equiv : RelationClasses.Equivalence eq := _.
+
+  Inductive lt_ : t -> t -> Prop :=
+  | lt_clause1 l e e' : LevelExpr.lt e e' -> lt_ (l, e) (l, e')
+  | lt_clause2 l l' b b' : LevelExprSet.lt l.(t_set) l'.(t_set) -> lt_ (l, b) (l', b').
+
+  Definition lt := lt_.
+
+  Global Instance lt_strorder : RelationClasses.StrictOrder lt.
+  Proof.
+    constructor.
+    - intros x X; inversion X; subst. now eapply LevelExpr.lt_strorder in H1.
+      eapply LevelExprSet.lt_strorder; eassumption.
+    - intros x y z X1 X2; invs X1; invs X2; constructor; tea.
+      etransitivity; tea.
+      etransitivity; tea.
+  Qed.
+
+  Definition lt_compat : Proper (Logic.eq ==> Logic.eq ==> iff) lt.
+    intros x x' H1 y y' H2. unfold lt. subst. reflexivity.
+  Qed.
+
+  Definition compare (x y : t) : comparison :=
+    match x, y with
+    | (l1, b1), (l2, b2) =>
+      match LevelExprSet.compare l1.(t_set) l2.(t_set) with
+      | Eq => LevelExpr.compare b1 b2
+      | x => x
+      end
+    end.
+
+  Definition compare_spec :
+    forall x y : t, CompareSpec (x = y) (lt x y) (lt y x) (compare x y).
+  Proof.
+    intros [? ?] [? ?]; cbn; repeat constructor.
+    destruct (LevelExprSet.compare_spec n n0); repeat constructor; tas.
+    eapply LevelExprSet.eq_leibniz in H. apply NonEmptySetFacts.eq_univ in H.
+    subst. cbn in *.
+    destruct (LevelExpr.compare_spec t0 t1); repeat constructor; tas. now subst.
+  Qed.
+
+  #[program] Global Instance reflect_eq_Z : ReflectEq Z := {
+    eqb := Z.eqb
+  }.
+  Next Obligation.
+    destruct (Z.eqb_spec x y); constructor => //.
+  Qed.
+
+  Global Instance reflect_t : ReflectEq t := reflect_prod _ _ .
+
+  Definition eq_dec : forall (l1 l2 : t), {l1 = l2} + {l1 <> l2} := Classes.eq_dec.
+
+  Definition eq_leibniz (x y : t) : eq x y -> x = y := id.
+
+  End Clause.
+
+  Module Clauses := MSetAVL.Make Clause.
+  Module ClausesFact := WFactsOn Clause Clauses.
+  Module ClausesProp := WPropertiesOn Clause Clauses.
+  Module ClausesDecide := WDecide (Clauses).
+  Ltac clsets := ClausesDecide.fsetdec.
+
+  Definition clauses := Clauses.t.
+
+  Lemma filter_add {p x s} : Clauses.Equal (Clauses.filter p (Clauses.add x s)) (if p x then Clauses.add x (Clauses.filter p s) else Clauses.filter p s).
+  Proof.
+    intros i.
+    rewrite Clauses.filter_spec.
+    destruct (eqb_spec i x); subst;
+    destruct (p x) eqn:px; rewrite !Clauses.add_spec !Clauses.filter_spec; intuition auto || congruence.
+  Qed.
+
+  Local Instance proper_fold_transpose {A} (f : Clauses.elt -> A -> A) :
+    transpose eq f ->
+    Proper (Clauses.Equal ==> eq ==> eq) (Clauses.fold f).
+  Proof.
+    intros hf s s' Hss' x ? <-.
+    eapply ClausesProp.fold_equal; tc; tea.
+  Qed.
+  Existing Class transpose.
+
+  Lemma clauses_fold_filter {A} (f : Clauses.elt -> A -> A) (p : Clauses.elt -> bool) cls acc :
+    transpose Logic.eq f ->
+    Clauses.fold f (Clauses.filter p cls) acc =
+    Clauses.fold (fun elt acc => if p elt then f elt acc else acc) cls acc.
+  Proof.
+    intros hf.
+    symmetry. eapply ClausesProp.fold_rec_bis.
+    - intros s s' a eq. intros ->.
+      eapply ClausesProp.fold_equal; tc. auto.
+      intros x.
+      rewrite !Clauses.filter_spec.
+      now rewrite eq.
+    - now cbn.
+    - intros.
+      rewrite H1.
+      rewrite filter_add.
+      destruct (p x) eqn:px => //.
+      rewrite ClausesProp.fold_add //.
+      rewrite Clauses.filter_spec. intuition auto.
+  Qed.
+
+  Definition strict_subset (s s' : LevelSet.t) :=
+    LevelSet.Subset s s' /\ ~ LevelSet.Equal s s'.
+
+  Lemma strict_subset_incl (x y z : LevelSet.t) : LevelSet.Subset x y -> strict_subset y z -> strict_subset x z.
+  Proof.
+    intros hs []. split => //. lsets.
+    intros heq. apply H0. lsets.
+  Qed.
+
+  Lemma strict_subset_cardinal s s' : strict_subset s s' -> LevelSet.cardinal s < LevelSet.cardinal s'.
+  Proof.
+    intros [].
+    assert (LevelSet.cardinal s <> LevelSet.cardinal s').
+    { intros heq. apply H0.
+      intros x. split; intros. now apply H.
+      destruct (LevelSet.mem x s) eqn:hin.
+      eapply LevelSet.mem_spec in hin.
+      auto. eapply LevelSetProp.FM.not_mem_iff in hin.
+      exfalso.
+      eapply LevelSetProp.subset_cardinal_lt in hin; tea.
+      lia. }
+    enough (LevelSet.cardinal s <= LevelSet.cardinal s') by lia.
+    now eapply LevelSetProp.subset_cardinal.
+  Qed.
+
+  Definition premise (cl : clause) := fst cl.
+  Definition concl (cl : clause) := snd cl.
+  Extraction Inline premise concl.
+
+  Definition clause_levels cl :=
+    LevelSet.union (levels (premise cl)) (LevelSet.singleton (level (concl cl))).
+
+  Definition clauses_levels (cls : clauses) : LevelSet.t :=
+    Clauses.fold (fun cl acc => LevelSet.union (clause_levels cl) acc) cls LevelSet.empty.
+
+  Lemma Clauses_In_elements l s :
+    In l (Clauses.elements s) <-> Clauses.In l s.
+  Proof.
+    rewrite ClausesFact.elements_iff.
+    now rewrite InA_In_eq.
+  Qed.
+
+  Lemma clauses_levels_spec_aux l cls acc :
+    LevelSet.In l (Clauses.fold (fun cl acc => LevelSet.union (clause_levels cl) acc) cls acc) <->
+    (exists cl, Clauses.In cl cls /\ LevelSet.In l (clause_levels cl)) \/ LevelSet.In l acc.
+  Proof.
+    eapply ClausesProp.fold_rec.
+    - intros.
+      intuition auto. destruct H1 as [k [hin hl]]. clsets.
+    - intros x a s' s'' hin nin hadd ih.
+      rewrite LevelSet.union_spec.
+      split.
+      * intros [hin'|].
+        left. exists x. split => //.
+        apply hadd. now left.
+        apply ih in H.
+        intuition auto.
+        left. destruct H0 as [k Hk]. exists k. intuition auto. apply hadd. now right.
+      * intros [[k [ins'' ?]]|inacc].
+        eapply hadd in ins''. destruct ins''; subst.
+        + now left.
+        + right. apply ih. now left; exists k.
+        + right. intuition auto.
+  Qed.
+
+  Lemma clauses_levels_spec l cls :
+    LevelSet.In l (clauses_levels cls) <->
+    exists cl, Clauses.In cl cls /\ LevelSet.In l (clause_levels cl).
+  Proof.
+    unfold clauses_levels.
+    rewrite clauses_levels_spec_aux.
+    intuition auto. lsets.
+  Qed.
+
+  Instance clauses_levels_proper : Proper (Clauses.Equal ==> LevelSet.Equal) clauses_levels.
+  Proof.
+    intros cl cl' eq x.
+    rewrite !clauses_levels_spec.
+    now setoid_rewrite eq.
+  Qed.
+
+  Lemma clause_levels_spec l cl :
+    LevelSet.In l (clause_levels cl) <->
+    LevelSet.In l (levels (premise cl)) \/ l = level (concl cl).
+  Proof.
+    unfold clause_levels.
+    now rewrite LevelSet.union_spec LevelSet.singleton_spec.
+  Qed.
+
+  Definition clause_conclusion cl := level (concl cl).
+End Clauses.
